theories/lang_oadt/inversion.v
@@ -66,44 +66,8 @@ Tactic Notation "kind_inv" "*" :=
 
 (** * Type inversion *)
 
-Module kernel.
-
-Section fix_gctx.
-
-Context (Σ : gctx).
-
-(** [TIte] and [TCase] require special rules. *)
-Inductive typing_inv : tctx -> expr -> llabel -> expr -> Prop :=
-| ITIte Γ l0 l1 l2 l e0 e1 e2 τ :
-    Γ ⊢ e0 :{l0} 𝔹 ->
-    Γ ⊢ e1 :{l1} τ^(lit true) ->
-    Γ ⊢ e2 :{l2} τ^(lit false) ->
-    l = l0 ⊔ l1 ⊔ l2 ->
-    forall l' τ',
-      l ⊑ l' ->
-      τ' ≡ <{ τ^e0 }> ->
-      typing_inv Γ <{ if e0 then e1 else e2 }> l' τ'
-| ITCase Γ l0 l1 l2 l e0 e1 e2 τ1 τ2 τ κ L1 L2 :
-    Γ ⊢ e0 :{l0} τ1 + τ2 ->
-    (forall x, x ∉ L1 -> Σ; <[x:=(l0, τ1)]>Γ ⊢ e1^x :{l1} τ^(inl<τ1 + τ2> x)) ->
-    (forall x, x ∉ L2 -> Σ; <[x:=(l0, τ2)]>Γ ⊢ e2^x :{l2} τ^(inr<τ1 + τ2> x)) ->
-    Γ ⊢ τ^e0 :: κ ->
-    l = l0 ⊔ l1 ⊔ l2 ->
-    forall l' τ',
-      l ⊑ l' ->
-      τ' ≡ <{ τ^e0 }> ->
-      typing_inv Γ <{ case e0 of e1 | e2 }> l' τ'
-.
-
-End fix_gctx.
-
-End kernel.
-
 Ltac tsf_typing ctor typing_inv :=
   lazymatch ctor with
-  (* Remove the cases about [TIte] and [TCase]. *)
-  | TIte => tsf_skip | TIteNoDep => tsf_skip
-  | TCase => tsf_skip | TCaseNoDep => tsf_skip
   | TConv => tsf_skip
   | _ =>
       let H := fresh in
@@ -112,49 +76,28 @@ Ltac tsf_typing ctor typing_inv :=
         lazymatch type of H with
         | forall e : ?T, _ =>
             refine (forall e : T, _ : Prop); specialize (H e)
-        | ?Σ; ?Γ ⊢ ?e :{?l} ?τ =>
-            let l' := fresh "l'" in
+        | ?Σ; ?Γ ⊢ ?e : ?τ =>
             let τ' := fresh "τ'" in
-            refine (forall (l' : llabel) (τ' : expr), _ : Prop);
-            lazymatch l with
-            | ⊤ => refine (l' = ⊤ -> _ : Prop)
-            | ⊥ => idtac
-            | _ => refine (l ⊑ l' -> _ : Prop)
-            end;
-            exact (Σ ⊢ τ' ≡ τ -> typing_inv Σ Γ e l' τ')
+            refine (forall (τ' : expr), _ : Prop);
+            exact (Σ ⊢ τ' ≡ τ -> typing_inv Σ Γ e τ')
         end
   end.
 
 MetaCoq Run (tsf_ind_gen_from
                typing "typing_inv"
-               (ltac:(tsf_ctors typing (append "I") tsf_typing) ++
-                ltac:(tsf_ctors_id kernel.typing_inv))).
+               ltac:(tsf_ctors typing (append "I") tsf_typing)).
 
 
-Lemma typing_inv_complete Σ Γ e l τ :
+Lemma typing_inv_complete Σ Γ e τ :
   gctx_wf Σ ->
-  Σ; Γ ⊢ e :{l} τ ->
-  typing_inv Σ Γ e l τ.
+  Σ; Γ ⊢ e : τ ->
+  typing_inv Σ Γ e τ.
 Proof.
   intros Hwf.
   induction 1; eauto using typing_inv with equiv_naive_solver.
 
-  (* TIte *)
-  - econstructor; eauto;
-    lazymatch goal with
-    | H : _ ⊢ _ : ?τ |- _ =>
-        rewrite (open_lc_intro τ) by eauto using typing_type_lc
-    end; eauto with equiv_naive_solver.
-
-  (* TCase *)
-  - econstructor; eauto; intros;
-    lazymatch goal with
-    | H : _ ⊢ ?τ :: _ |- _ =>
-        rewrite (open_lc_intro τ) by eauto using kinding_lc
-    end; eauto with equiv_naive_solver.
-
   (* TConv *)
-  - select (typing_inv _ _ _ _ _) (fun H => sinvert H);
+  - select (typing_inv _ _ _ _) (fun H => sinvert H);
     econstructor; subst;
     eauto using (top_inv (A:=bool)) with equiv_naive_solver lattice_naive_solver.
 Qed.
