theories/lang_oadt/semantics.v
@@ -5,27 +5,6 @@ Implicit Types (b : bool).
 
 (** * Definitions *)
 
-(** ** Weak values *)
-Inductive wval : expr -> Prop :=
-| WLit b : wval <{ lit b }>
-| WPair v1 v2 : wval v1 -> wval v2 -> wval <{ (v1, v2) }>
-| WAbs l τ e : wval <{ \:{l}τ => e }>
-| WInj b τ v : wval v -> wval <{ inj@b<τ> v }>
-| WFold X v : wval v -> wval <{ fold<X> v }>
-| WIte b v1 v2 :
-    wval v1 -> wval v2 ->
-    wval <{ ~if [b] then v1 else v2 }>
-| WOVal v : oval v -> wval v
-.
-
-(** ** Weak oblivious values *)
-Inductive woval : expr -> Prop :=
-| OWIte b v1 v2 :
-    woval v1 -> woval v2 ->
-    woval <{ ~if [b] then v1 else v2 }>
-| OWOVal v : oval v -> woval v
-.
-
 (** ** OADT value typing *)
 (** [ovalty v ω] means [v] is an oblivious value of oblivious type value [ω].
 This is essentially a subset of [typing], but we have it so that the dynamic
@@ -34,13 +13,13 @@ Inductive ovalty : expr -> expr -> Prop :=
 | OTUnit : ovalty <{ () }> <{ 𝟙 }>
 | OTOBool b : ovalty <{ [b] }> <{ ~𝔹 }>
 | OTProd v1 v2 ω1 ω2 :
-    ovalty v1 ω1 -> ovalty v2 ω2 ->
-    ovalty <{ ~(v1, v2) }> <{ ω1 ~* ω2 }>
+  ovalty v1 ω1 -> ovalty v2 ω2 ->
+  ovalty <{ ~(v1, v2) }> <{ ω1 ~* ω2 }>
 | OTOSum b v ω1 ω2 :
-    ovalty v <{ ite b ω1 ω2 }> ->
-    (* Make sure the unused oblivious type is a value. *)
-    otval <{ ite b ω2 ω1 }> ->
-    ovalty <{ [inj@b<ω1 ~+ ω2> v] }> <{ ω1 ~+ ω2 }>
+  ovalty v <{ ite b ω1 ω2 }> ->
+  (* Make sure the unused oblivious type is a value. *)
+  otval <{ ite b ω2 ω1 }> ->
+  ovalty <{ [inj@b<ω1 ~+ ω2> v] }> <{ ω1 ~+ ω2 }>
 .
 
 (** ** Evaluation context (ℇ) *)
@@ -55,16 +34,13 @@ Variant ectx : (expr -> expr) -> Prop :=
 | CtxOSum1 τ2 : ectx (fun τ1 => <{ τ1 ~+ τ2 }>)
 | CtxOSum2 ω1 : otval ω1 -> ectx (fun τ2 => <{ ω1 ~+ τ2 }>)
 | CtxApp1 e2 : ectx (fun e1 => <{ e1 e2 }>)
-| CtxApp2 v1 : wval v1 -> ectx (fun e2 => <{ v1 e2 }>)
+| CtxApp2 v1 : val v1 -> ectx (fun e2 => <{ v1 e2 }>)
 | CtxTApp X : ectx (fun e => <{ X@e }>)
 | CtxLet e2 : ectx (fun e1 => <{ let e1 in e2 }>)
 | CtxSec : ectx (fun e => <{ s𝔹 e }>)
 | CtxIte e1 e2 : ectx (fun e0 => <{ if e0 then e1 else e2 }>)
-| CtxOIte1 e1 e2 : ectx (fun e0 => <{ ~if e0 then e1 else e2 }>)
-| CtxOIte2 v0 e2 : wval v0 -> ectx (fun e1 => <{ ~if v0 then e1 else e2 }>)
-| CtxOIte3 v0 v1 : wval v0 -> wval v1 -> ectx (fun e2 => <{ ~if v0 then v1 else e2 }>)
 | CtxPair1 l e2 : ectx (fun e1 => <{ (e1, e2){l} }>)
-| CtxPair2 l v1 : wval v1 -> ectx (fun e2 => <{ (v1, e2){l} }>)
+| CtxPair2 l v1 : val v1 -> ectx (fun e2 => <{ (v1, e2){l} }>)
 | CtxProj l b : ectx (fun e => <{ π{l}@b e }>)
 | CtxInj b τ : ectx (fun e => <{ inj@b<τ> e }>)
 | CtxOInj1 b e : ectx (fun τ => <{ ~inj@b<τ> e }>)
@@ -73,22 +49,10 @@ Variant ectx : (expr -> expr) -> Prop :=
 | CtxOCase e1 e2: ectx (fun e0 => <{ ~case e0 of e1 | e2 }>)
 | CtxFold X : ectx (fun e => <{ fold<X> e }>)
 | CtxUnfold X : ectx (fun e => <{ unfold<X> e }>)
-| CtxTape : ectx (fun e => <{ tape e }>)
 | CtxMux1 e1 e2 : ectx (fun e0 => <{ mux e0 e1 e2 }>)
-| CtxMux2 v0 e2 : wval v0 -> ectx (fun e1 => <{ mux v0 e1 e2 }>)
-| CtxMux3 v0 v1 : wval v0 -> wval v1 -> ectx (fun e2 => <{ mux v0 v1 e2 }>)
+| CtxMux2 v0 e2 : val v0 -> ectx (fun e1 => <{ mux v0 e1 e2 }>)
+| CtxMux3 v0 v1 : val v0 -> val v1 -> ectx (fun e2 => <{ mux v0 v1 e2 }>)
 .
-
-(** The evaluation context enclosing possibly leaking expressions. *)
-Variant lectx : (expr -> expr) -> Prop :=
-| LCtxApp v2 : wval v2 -> lectx (fun e1 => <{ e1 v2 }>)
-| LCtxSec : lectx (fun e => <{ s𝔹 e }>)
-| LCtxIte e1 e2 : lectx (fun e0 => <{ if e0 then e1 else e2 }>)
-| LCtxProj b : lectx (fun e => <{ π@b e }>)
-| LCtxCase e1 e2: lectx (fun e0 => <{ case e0 of e1 | e2 }>)
-| LCtxUnfold X : lectx (fun e => <{ unfold<X> e }>)
-.
-
 
 (** ** Small-step relation *)
 Section step.
@@ -98,60 +62,49 @@ Context (Σ : gctx).
 Reserved Notation "e '-->!' e'" (at level 40).
 
 Inductive step : expr -> expr -> Prop :=
-| SApp l τ e v :
-    wval v ->
-    <{ (\:{l}τ => e) v }> -->! <{ e^v }>
+| SApp τ e v :
+  val v ->
+  <{ (\:τ => e) v }> -->! <{ e^v }>
 | STApp X τ' τ v :
-    wval v ->
-    Σ !! X = Some (DOADT τ' τ) ->
-    <{ X@v }> -->! <{ τ^v }>
+  val v ->
+  Σ !! X = Some (DOADT τ' τ) ->
+  <{ X@v }> -->! <{ τ^v }>
 | SFun x T e :
-    Σ !! x = Some (DFun T e) ->
-    <{ gvar x }> -->! <{ e }>
+  Σ !! x = Some (DFun T e) ->
+  <{ gvar x }> -->! <{ e }>
 | SLet v e :
-    wval v ->
-    <{ let v in e }> -->! <{ e^v }>
+  val v ->
+  <{ let v in e }> -->! <{ e^v }>
 | SSec b :
-    <{ s𝔹 b }> -->! <{ [b] }>
+  <{ s𝔹 b }> -->! <{ [b] }>
 | SIte b e1 e2 :
-    <{ if b then e1 else e2 }> -->! <{ ite b e1 e2 }>
+  <{ if b then e1 else e2 }> -->! <{ ite b e1 e2 }>
 | SProj l b v1 v2 :
-    wval v1 -> wval v2 ->
-    <{ π{l}@b (v1, v2){l} }> -->! <{ ite b v1 v2 }>
+  val v1 -> val v2 ->
+  <{ π{l}@b (v1, v2){l} }> -->! <{ ite b v1 v2 }>
 | SOInj b ω v :
-    otval ω -> oval v ->
-    <{ ~inj@b<ω> v }> -->! <{ [inj@b<ω> v] }>
+  otval ω -> oval v ->
+  <{ ~inj@b<ω> v }> -->! <{ [inj@b<ω> v] }>
 | SCase b τ v e1 e2 :
-    wval v ->
-    <{ case inj@b<τ> v of e1 | e2 }> -->! <{ ite b (e1^v) (e2^v) }>
+  val v ->
+  <{ case inj@b<τ> v of e1 | e2 }> -->! <{ ite b (e1^v) (e2^v) }>
 (* One of the most interesting rules. *)
 | SOCase b ω1 ω2 v e1 e2 v1 v2 :
-    oval v ->
-    ovalty v1 ω1 -> ovalty v2 ω2 ->
-    <{ ~case [inj@b<ω1 ~+ ω2> v] of e1 | e2 }> -->!
-      <{ ~if [b] then (ite b (e1^v) (e1^v1)) else (ite b (e2^v2) (e2^v)) }>
+  oval v ->
+  ovalty v1 ω1 -> ovalty v2 ω2 ->
+  <{ ~case [inj@b<ω1 ~+ ω2> v] of e1 | e2 }> -->!
+  <{ mux [b] (ite b (e1^v) (e1^v1)) (ite b (e2^v2) (e2^v)) }>
 | SUnfold X X' v :
-    wval v ->
-    <{ unfold<X> (fold <X'> v) }> -->! v
+  val v ->
+  <{ unfold<X> (fold <X'> v) }> -->! v
 | SMux b v1 v2 :
-    wval v1 -> wval v2 ->
-    <{ mux [b] v1 v2 }> -->! <{ ite b v1 v2 }>
-| STapeOIte b v1 v2 :
-    woval v1 -> woval v2 ->
-    <{ tape (~if [b] then v1 else v2) }> -->! <{ mux [b] (tape v1) (tape v2) }>
-(* [tape v] is a no-op if [v] is an oblivious value. *)
-| STapeOVal v :
-    oval v ->
-    <{ tape v }> -->! <{ v }>
-| SOIte b v1 v2 ℇ :
-    lectx ℇ ->
-    wval v1 -> wval v2 ->
-    ℇ <{ ~if [b] then v1 else v2 }> -->! <{ ~if [b] then ,(ℇ v1) else ,(ℇ v2) }>
+  val v1 -> val v2 ->
+  <{ mux [b] v1 v2 }> -->! <{ ite b v1 v2 }>
 (* Step under evaluation context *)
 | SCtx ℇ e e' :
-    ectx ℇ ->
-    e -->! e' ->
-    ℇ e -->! ℇ e'
+  ectx ℇ ->
+  e -->! e' ->
+  ℇ e -->! ℇ e'
 
 where "e '-->!' e'" := (step e e').
 
