theories/lang_oadt/syntax.v
@@ -14,16 +14,6 @@ Notation olabel := bool (only parsing).
 Notation LObliv := true (only parsing).
 Notation LPub := false (only parsing).
 
-(** ** Leakage label *)
-(** Defined as alias of [bool]. A leaky expression (with [LLeak] label) may contain
-potential leaks, and a safe expression (with [LSafe] label) doesn't. A leaky
-expression need to be "fixed" by the [tape] construct in order for obliviousness
-and they can not interfere types. We may use [⊤] for [LLeak] and [⊥] for
-[LSafe]. *)
-Notation llabel := bool (only parsing).
-Notation LLeak := true (only parsing).
-Notation LSafe := false (only parsing).
-
 (** ** Expressions (e, τ) *)
 (** We use locally nameless representation for binders. *)
 Inductive expr :=
@@ -34,8 +24,8 @@ Inductive expr :=
 (* Global variables, referring to global functions, ADTs and OADTs. *)
 | EGVar (x : atom)
 (* Functions *)
-| EPi (l : llabel) (τ1 τ2: expr)
-| EAbs (l : llabel) (τ e : expr)
+| EPi (τ1 τ2: expr)
+| EAbs (τ e : expr)
 | EApp (e1 e2 : expr)
 (* Oblivious type application *)
 | ETApp (X : atom) (e : expr)
@@ -49,8 +39,8 @@ Inductive expr :=
 | ELit (b : bool)
 (* Boolean section *)
 | ESec (e : expr)
-(* Public and oblivious conditional. The oblivious conditional may be leaky *)
-| EIte (l : olabel) (e0 e1 e2 : expr)
+(* Public conditional. *)
+| EIte (e0 e1 e2 : expr)
 (* Public and oblivious product, pair and projection. Technically we do not need
 to distinguish bewteen public and oblivious product, but this is conceptually
 cleaner in my opinion. It also makes certain aspects of semantics and type
@@ -59,19 +49,14 @@ and elaborated, so the surface language needs not distinguish them. *)
 | EProd (l : olabel) (τ1 τ2 : expr)
 | EPair (l : olabel) (e1 e2 : expr)
 | EProj (l : olabel) (b : bool) (e : expr)
-(* Public and oblivious sum, injection and case analysis. The oblivious case may
-be leaky. *)
+(* Public and oblivious sum, injection and case analysis. *)
 | ESum (l : olabel) (τ1 τ2 : expr)
 | EInj (l : olabel) (b : bool) (τ e : expr)
 | ECase (l : olabel) (e0 : expr) (e1 : expr) (e2 : expr)
 (* Introduction and elimination of ADTs *)
 | EFold (X : atom) (e : expr)
 | EUnfold (X : atom) (e : expr)
-(* Tape the leakage. *)
-| ETape (e : expr)
-(* Oblivious conditional, i.e. MUX. Technically we do not need this in the
-source language, but it is a convenient machinery for a conceptually cleaner
-semantics. *)
+(* Oblivious conditional, i.e. MUX. *)
 | EMux (e0 e1 e2 : expr)
 (* Runtime expressions *)
 | EBoxedLit (b : bool)
@@ -85,18 +70,11 @@ Proof.
   solve_decision.
 Defined.
 
-(** ** Expressions with leakage label (T) *)
-Definition lexpr := (llabel * expr).
-Definition lexpr_label : lexpr -> llabel := fst.
-Arguments lexpr_label /.
-Definition lexpr_expr : lexpr -> expr := snd.
-Arguments lexpr_expr /.
-
 (** ** Global definitions (D) *)
 Variant gdef :=
 | DADT (e : expr)
 | DOADT (τ e : expr)
-| DFun (T : lexpr) (e : expr)
+| DFun (t : expr) (e : expr)
 .
 
 (** ** Global context (Σ) *)
@@ -120,7 +98,6 @@ Module expr_notations.
 
 (* Adapted from _Software Foundations_. *)
 Coercion ELit : bool >-> expr.
-Coercion lexpr_expr : lexpr >-> expr.
 
 (** Quote *)
 Notation "<{ e }>" := e (e custom oadt at level 99).
@@ -132,63 +109,43 @@ Notation "( x )" := x (in custom oadt, x at level 99).
 Notation "x" := x (in custom oadt at level 0, x constr at level 0).
 Notation "'bvar' x" := (EBVar x) (in custom oadt at level 0, x constr at level 0).
 Notation "'fvar' x" := (EFVar x) (in custom oadt at level 0, x constr at level 0,
-                                     only parsing).
+                             only parsing).
 Notation "'gvar' x" := (EGVar x) (in custom oadt at level 0, x constr at level 0).
 Notation "'lit' b" := (ELit b) (in custom oadt at level 0, b constr at level 0,
-                                   only parsing).
+                            only parsing).
 Notation "'𝟙'" := EUnitT (in custom oadt at level 0).
 Notation "'Unit'" := EUnitT (in custom oadt at level 0, only parsing).
 Notation "'𝔹{' l '}'" := (EBool l) (in custom oadt at level 0,
-                                       l constr at level 0,
-                                       format "'𝔹{' l '}'").
+                               l constr at level 0,
+                               format "'𝔹{' l '}'").
 Notation "'𝔹'" := (EBool LPub) (in custom oadt at level 0).
 Notation "'Bool'" := (EBool LPub) (in custom oadt at level 0, only parsing).
 Notation "'~𝔹'" := (EBool LObliv) (in custom oadt at level 0).
 Notation "'~Bool'" := (EBool LObliv) (in custom oadt at level 0, only parsing).
 Notation "τ1 '*{' l '}' τ2" := (EProd l τ1 τ2) (in custom oadt at level 3,
-                                                   l constr at level 0,
-                                                   τ1 custom oadt,
-                                                   τ2 custom oadt at level 0,
-                                                  format "τ1  '*{' l '}'  τ2").
+                                     l constr at level 0,
+                                     τ1 custom oadt,
+                                     τ2 custom oadt at level 0,
+                                     format "τ1  '*{' l '}'  τ2").
 Notation "τ1 * τ2" := (EProd LPub τ1 τ2) (in custom oadt at level 3,
-                                             τ1 custom oadt,
-                                             τ2 custom oadt at level 0).
+                            τ1 custom oadt,
+                            τ2 custom oadt at level 0).
 Notation "τ1 ~* τ2" := (EProd LObliv τ1 τ2) (in custom oadt at level 3,
-                                                τ1 custom oadt,
-                                                τ2 custom oadt at level 0).
+                             τ1 custom oadt,
+                             τ2 custom oadt at level 0).
 Notation "τ1 '+{' l '}' τ2" := (ESum l τ1 τ2) (in custom oadt at level 4,
-                                                  l constr at level 0,
-                                                  left associativity,
-                                                  format "τ1  '+{' l '}'  τ2").
+                                     l constr at level 0,
+                                     left associativity,
+                                     format "τ1  '+{' l '}'  τ2").
 Notation "τ1 + τ2" := (ESum LPub τ1 τ2) (in custom oadt at level 4,
-                                            left associativity).
+                            left associativity).
 Notation "τ1 ~+ τ2" := (ESum LObliv τ1 τ2) (in custom oadt at level 4,
-                                               left associativity).
-Notation "'Π' :{ l } τ1 , τ2" := (EPi l τ1 τ2)
-                                   (in custom oadt at level 50,
-                                       right associativity,
-                                       format "Π :{ l } τ1 ,  τ2").
-Notation "'Π' !: τ1 , τ2" := (EPi LSafe τ1 τ2)
-                               (in custom oadt at level 50,
-                                   right associativity,
-                                   format "Π !: τ1 ,  τ2").
-Notation "'Π' : τ1 , τ2" := (EPi LLeak τ1 τ2)
+                             left associativity).
+Notation "'Π' : τ1 , τ2" := (EPi τ1 τ2)
                               (in custom oadt at level 50,
                                   right associativity,
                                   format "Π : τ1 ,  τ2").
-Notation "\ :{ l } τ '=>' e" := (EAbs l τ e)
-                                  (in custom oadt at level 90,
-                                      τ custom oadt at level 99,
-                                      e custom oadt at level 99,
-                                      left associativity,
-                                      format "\ :{ l } τ  =>  e").
-Notation "\ !: τ '=>' e" := (EAbs LSafe τ e)
-                              (in custom oadt at level 90,
-                                  τ custom oadt at level 99,
-                                  e custom oadt at level 99,
-                                  left associativity,
-                                  format "\ !: τ  =>  e").
-Notation "\ : τ '=>' e" := (EAbs LLeak τ e)
+Notation "\ : τ '=>' e" := (EAbs τ e)
                              (in custom oadt at level 90,
                                  τ custom oadt at level 99,
                                  e custom oadt at level 99,
@@ -196,7 +153,7 @@ Notation "\ : τ '=>' e" := (EAbs LLeak τ e)
                                  format "\ : τ  =>  e").
 Notation "e1 e2" := (EApp e1 e2) (in custom oadt at level 2, left associativity).
 Notation "X @ e" := (ETApp X e) (in custom oadt at level 2,
-                                    format "X @ e").
+                          format "X @ e").
 Notation "()" := EUnitV (in custom oadt at level 0).
 Notation "( x , y , .. , z ){ l }" := (EPair l .. (EPair l x y) .. z)
                                         (in custom oadt at level 0,
@@ -217,105 +174,91 @@ Notation "~( x , y , .. , z )" := (EPair LObliv .. (EPair LObliv x y) .. z)
                                         z custom oadt at level 99,
                                         format "~( x ,  y ,  .. ,  z )").
 Notation "'π{' l '}@' b e" := (EProj l b e) (in custom oadt at level 2,
-                                              l constr at level 0,
-                                              b constr at level 0,
-                                              format "π{ l }@ b  e").
+                                    l constr at level 0,
+                                    b constr at level 0,
+                                    format "π{ l }@ b  e").
 Notation "'π@' b e" := (EProj LPub b e) (in custom oadt at level 2,
-                                            b constr at level 0,
-                                            format "π@ b  e").
+                             b constr at level 0,
+                             format "π@ b  e").
 Notation "'~π@' b e" := (EProj LObliv b e) (in custom oadt at level 2,
-                                               b constr at level 0,
-                                               format "~π@ b  e").
+                              b constr at level 0,
+                              format "~π@ b  e").
 Notation "'π1' e" := (EProj LPub true e) (in custom oadt at level 2).
 Notation "'π2' e" := (EProj LPub false e) (in custom oadt at level 2).
 Notation "'~π1' e" := (EProj LObliv true e) (in custom oadt at level 2).
 Notation "'~π2' e" := (EProj LObliv false e) (in custom oadt at level 2).
 Notation "'s𝔹' e" := (ESec e) (in custom oadt at level 2).
-Notation "'if{' l '}' e0 'then' e1 'else' e2" := (EIte l e0 e1 e2)
-                                                   (in custom oadt at level 89,
-                                                       l constr at level 0,
-                                                       e0 custom oadt at level 99,
-                                                       e1 custom oadt at level 99,
-                                                       e2 custom oadt at level 99,
-                                                       left associativity,
-                                                       format "'if{' l '}'  e0  'then'  e1  'else'  e2").
-Notation "'if' e0 'then' e1 'else' e2" := (EIte LPub e0 e1 e2)
+Notation "'if' e0 'then' e1 'else' e2" := (EIte e0 e1 e2)
                                             (in custom oadt at level 89,
                                                 e0 custom oadt at level 99,
                                                 e1 custom oadt at level 99,
                                                 e2 custom oadt at level 99,
                                                 left associativity).
-Notation "'~if' e0 'then' e1 'else' e2" := (EIte LObliv e0 e1 e2)
-                                             (in custom oadt at level 89,
-                                                 e0 custom oadt at level 99,
-                                                 e1 custom oadt at level 99,
-                                                 e2 custom oadt at level 99).
 Notation "'let' e1 'in' e2" := (ELet e1 e2)
                                  (in custom oadt at level 0,
                                      e1 custom oadt at level 99,
                                      e2 custom oadt at level 99).
 Notation "'inj{' l '}@' b < τ > e" := (EInj l b τ e) (in custom oadt at level 2,
-                                                         l constr at level 0,
-                                                         b constr at level 0,
-                                                         τ custom oadt at level 0,
-                                                         format "'inj{' l '}@' b < τ >  e").
+                                            l constr at level 0,
+                                            b constr at level 0,
+                                            τ custom oadt at level 0,
+                                            format "'inj{' l '}@' b < τ >  e").
 Notation "'inl{' l '}' < τ > e" := (EInj l true τ e) (in custom oadt at level 2,
-                                                         τ custom oadt at level 0,
-                                                         format "inl{ l } < τ >  e").
+                                         τ custom oadt at level 0,
+                                         format "inl{ l } < τ >  e").
 Notation "'inr{' l '}' < τ > e" := (EInj l false τ e) (in custom oadt at level 2,
-                                                          τ custom oadt at level 0,
-                                                          format "inr{ l } < τ >  e").
+                                         τ custom oadt at level 0,
+                                         format "inr{ l } < τ >  e").
 Notation "'inj@' b < τ > e" := (EInj LPub b τ e) (in custom oadt at level 2,
-                                                     b constr at level 0,
-                                                     τ custom oadt at level 0,
-                                                     format "inj@ b < τ >  e").
+                                     b constr at level 0,
+                                     τ custom oadt at level 0,
+                                     format "inj@ b < τ >  e").
 Notation "'inl' < τ > e" := (EInj LPub true τ e) (in custom oadt at level 2,
-                                                     τ custom oadt at level 0,
-                                                     format "inl < τ >  e").
+                                  τ custom oadt at level 0,
+                                  format "inl < τ >  e").
 Notation "'inr' < τ > e" := (EInj LPub false τ e) (in custom oadt at level 2,
-                                                      τ custom oadt at level 0,
-                                                      format "inr < τ >  e").
+                                  τ custom oadt at level 0,
+                                  format "inr < τ >  e").
 Notation "'~inj@' b < τ > e" := (EInj LObliv b τ e) (in custom oadt at level 2,
-                                                        b constr at level 0,
-                                                        τ custom oadt at level 0,
-                                                        format "~inj@ b < τ >  e").
+                                      b constr at level 0,
+                                      τ custom oadt at level 0,
+                                      format "~inj@ b < τ >  e").
 Notation "'~inl' < τ > e" := (EInj LObliv true τ e) (in custom oadt at level 2,
-                                                        τ custom oadt at level 0,
-                                                        format "~inl < τ >  e").
+                                   τ custom oadt at level 0,
+                                   format "~inl < τ >  e").
 Notation "'~inr' < τ > e" := (EInj LObliv false τ e) (in custom oadt at level 2,
-                                                         τ custom oadt at level 0,
-                                                         format "~inr < τ >  e").
+                                   τ custom oadt at level 0,
+                                   format "~inr < τ >  e").
 Notation "'case{' l '}' e0 'of' e1 '|' e2" :=
   (ECase l e0 e1 e2) (in custom oadt at level 89,
-                         l constr at level 0,
-                         e0 custom oadt at level 99,
-                         e1 custom oadt at level 99,
-                         e2 custom oadt at level 99,
-                         left associativity,
-                         format "'case{' l '}'  e0  'of'  e1  '|'  e2").
+        l constr at level 0,
+        e0 custom oadt at level 99,
+        e1 custom oadt at level 99,
+        e2 custom oadt at level 99,
+        left associativity,
+        format "'case{' l '}'  e0  'of'  e1  '|'  e2").
 Notation "'case' e0 'of' e1 '|' e2" :=
   (ECase LPub e0 e1 e2) (in custom oadt at level 89,
-                            e0 custom oadt at level 99,
-                            e1 custom oadt at level 99,
-                            e2 custom oadt at level 99,
-                            left associativity).
+        e0 custom oadt at level 99,
+        e1 custom oadt at level 99,
+        e2 custom oadt at level 99,
+        left associativity).
 Notation "'~case' e0 'of' e1 '|' e2" :=
   (ECase LObliv e0 e1 e2) (in custom oadt at level 89,
-                              e0 custom oadt at level 99,
-                              e1 custom oadt at level 99,
-                              e2 custom oadt at level 99,
-                              left associativity).
+        e0 custom oadt at level 99,
+        e1 custom oadt at level 99,
+        e2 custom oadt at level 99,
+        left associativity).
 Notation "'fold' < X > e" := (EFold X e) (in custom oadt at level 2,
-                                             X custom oadt at level 0,
-                                             format "fold < X >  e").
+                                   X custom oadt at level 0,
+                                   format "fold < X >  e").
 Notation "'unfold' < X > e" := (EUnfold X e) (in custom oadt at level 2,
-                                                 X custom oadt at level 0,
-                                                 format "unfold < X >  e").
-Notation "'tape' e" := (ETape e) (in custom oadt at level 2).
+                                     X custom oadt at level 0,
+                                     format "unfold < X >  e").
 Notation "'mux' e0 e1 e2" := (EMux e0 e1 e2) (in custom oadt at level 2,
-                                                 e0 custom oadt at level 0,
-                                                 e1 custom oadt at level 0,
-                                                 e2 custom oadt at level 0).
+                                   e0 custom oadt at level 0,
+                                   e1 custom oadt at level 0,
+                                   e2 custom oadt at level 0).
 
 Notation "[ b ]" := (EBoxedLit b) (in custom oadt at level 0,
                                       b constr at level 0).
@@ -342,9 +285,6 @@ Notation "'ite' e0 e1 e2" := (if e0 then e1 else e2)
                                    e1 custom oadt at level 0,
                                    e2 custom oadt at level 0).
 
-(** Boolean retraction. *)
-Notation "'r𝔹' e" := <{ ~if e then true else false }> (in custom oadt at level 2).
-
 End expr_notations.
 
 
@@ -361,15 +301,15 @@ Reserved Notation "'{' k '~>' s '}' e" (in custom oadt at level 20, k constr).
 Fixpoint open_ (k : nat) (s : expr) (e : expr) : expr :=
   match e with
   | <{ bvar n }> => if decide (k = n) then s else e
-  | <{ Π:{l}τ1, τ2 }> => <{ Π:{l}({k~>s}τ1), {S k~>s}τ2 }>
-  | <{ \:{l}τ => e }> => <{ \:{l}({k~>s}τ) => {S k~>s}e }>
+  | <{ Π:τ1, τ2 }> => <{ Π:({k~>s}τ1), {S k~>s}τ2 }>
+  | <{ \:τ => e }> => <{ \:({k~>s}τ) => {S k~>s}e }>
   | <{ let e1 in e2 }> => <{ let {k~>s}e1 in {S k~>s}e2 }>
   | <{ case{l} e0 of e1 | e2 }> => <{ case{l} {k~>s}e0 of {S k~>s}e1 | {S k~>s}e2 }>
   (* Congruence rules *)
   | <{ e1 e2 }> => <{ ({k~>s}e1) ({k~>s}e2) }>
   | <{ X@e }> => <{ X@({k~>s}e) }>
   | <{ s𝔹 e }> => <{ s𝔹 ({k~>s}e) }>
-  | <{ if{l} e0 then e1 else e2 }> => <{ if{l} {k~>s}e0 then {k~>s}e1 else {k~>s}e2 }>
+  | <{ if e0 then e1 else e2 }> => <{ if {k~>s}e0 then {k~>s}e1 else {k~>s}e2 }>
   | <{ τ1 *{l} τ2 }> => <{ ({k~>s}τ1) *{l} ({k~>s}τ2) }>
   | <{ (e1, e2){l} }> => <{ ({k~>s}e1, {k~>s}e2){l} }>
   | <{ π{l}@b e }> => <{ π{l}@b ({k~>s}e) }>
@@ -377,7 +317,6 @@ Fixpoint open_ (k : nat) (s : expr) (e : expr) : expr :=
   | <{ inj{l}@b<τ> e }> => <{ inj{l}@b<({k~>s}τ)> ({k~>s}e) }>
   | <{ fold<X> e }> => <{ fold<X> ({k~>s}e) }>
   | <{ unfold<X> e }> => <{ unfold<X> ({k~>s}e) }>
-  | <{ tape e }> => <{ tape ({k~>s}e) }>
   | <{ mux e0 e1 e2 }> => <{ mux ({k~>s}e0) ({k~>s}e1) ({k~>s}e2) }>
   | _ => e
   end
@@ -394,13 +333,13 @@ Fixpoint subst (x : atom) (s : expr) (e : expr) : expr :=
   match e with
   | <{ fvar y }> => if decide (x = y) then s else e
   (* Congruence rules *)
-  | <{ Π:{l}τ1, τ2 }> => <{ Π:{l}({x↦s}τ1), {x↦s}τ2 }>
-  | <{ \:{l}τ => e }> => <{ \:{l}({x↦s}τ) => {x↦s}e }>
+  | <{ Π:τ1, τ2 }> => <{ Π:({x↦s}τ1), {x↦s}τ2 }>
+  | <{ \:τ => e }> => <{ \:({x↦s}τ) => {x↦s}e }>
   | <{ e1 e2 }> => <{ ({x↦s}e1) ({x↦s}e2) }>
   | <{ X@e }> => <{ X@({x↦s}e) }>
   | <{ let e1 in e2 }> => <{ let {x↦s}e1 in {x↦s}e2 }>
   | <{ s𝔹 e }> => <{ s𝔹 ({x↦s}e) }>
-  | <{ if{l} e0 then e1 else e2 }> => <{ if{l} {x↦s}e0 then {x↦s}e1 else {x↦s}e2 }>
+  | <{ if e0 then e1 else e2 }> => <{ if {x↦s}e0 then {x↦s}e1 else {x↦s}e2 }>
   | <{ τ1 *{l} τ2 }> => <{ ({x↦s}τ1) *{l} ({x↦s}τ2) }>
   | <{ (e1, e2){l} }> => <{ ({x↦s}e1, {x↦s}e2){l} }>
   | <{ π{l}@b e }> => <{ π{l}@b ({x↦s}e) }>
@@ -409,14 +348,11 @@ Fixpoint subst (x : atom) (s : expr) (e : expr) : expr :=
   | <{ case{l} e0 of e1 | e2 }> => <{ case{l} {x↦s}e0 of {x↦s}e1 | {x↦s}e2 }>
   | <{ fold<X> e }> => <{ fold<X> ({x↦s}e) }>
   | <{ unfold<X> e }> => <{ unfold<X> ({x↦s}e) }>
-  | <{ tape e }> => <{ tape ({x↦s}e) }>
   | <{ mux e0 e1 e2 }> => <{ mux ({x↦s}e0) ({x↦s}e1) ({x↦s}e2) }>
   | _ => e
   end
 
 where "'{' x '↦' s '}' e" := (subst x s e) (in custom oadt).
-
-Definition lexpr_subst x s (T : lexpr) := (T.1, subst x s T.2).
 
 (** ** Oblivious type values (ω) *)
 Inductive otval : expr -> Prop :=
@@ -438,7 +374,7 @@ Inductive oval : expr -> Prop :=
 Inductive val : expr -> Prop :=
 | VLit b : val <{ lit b }>
 | VPair v1 v2 : val v1 -> val v2 -> val <{ (v1, v2) }>
-| VAbs l τ e : val <{ \:{l}τ => e }>
+| VAbs τ e : val <{ \:τ => e }>
 | VInj b τ v : val v -> val <{ inj@b<τ> v }>
 | VFold X v : val v -> val <{ fold<X> v }>
 | VOVal v : oval v -> val v
@@ -448,19 +384,19 @@ Inductive val : expr -> Prop :=
 Inductive lc : expr -> Prop :=
 | LCFVar x : lc <{ fvar x }>
 | LCGVar x : lc <{ gvar x }>
-| LCPi l τ1 τ2 L :
-    (forall x, x ∉ L -> lc <{ τ2^x }>) ->
-    lc τ1 -> lc <{ Π:{l}τ1, τ2 }>
-| LCAbs l τ e L :
-    (forall x, x ∉ L -> lc <{ e^x }>) ->
-    lc τ -> lc <{ \:{l}τ => e }>
+| LCPi τ1 τ2 L :
+  (forall x, x ∉ L -> lc <{ τ2^x }>) ->
+  lc τ1 -> lc <{ Π:τ1, τ2 }>
+| LCAbs τ e L :
+  (forall x, x ∉ L -> lc <{ e^x }>) ->
+  lc τ -> lc <{ \:τ => e }>
 | LCLet e1 e2 L :
-    (forall x, x ∉ L -> lc <{ e2^x }>) ->
-    lc e1 -> lc <{ let e1 in e2 }>
+  (forall x, x ∉ L -> lc <{ e2^x }>) ->
+  lc e1 -> lc <{ let e1 in e2 }>
 | LCCase l e0 e1 e2 L1 L2 :
-    (forall x, x ∉ L1 -> lc <{ e1^x }>) ->
-    (forall x, x ∉ L2 -> lc <{ e2^x }>) ->
-    lc e0 -> lc <{ case{l} e0 of e1 | e2 }>
+  (forall x, x ∉ L1 -> lc <{ e1^x }>) ->
+  (forall x, x ∉ L2 -> lc <{ e2^x }>) ->
+  lc e0 -> lc <{ case{l} e0 of e1 | e2 }>
 (* Congruence rules *)
 | LCUnitT : lc <{ 𝟙 }>
 | LCUnitV : lc <{ () }>
@@ -469,7 +405,7 @@ Inductive lc : expr -> Prop :=
 | LCTApp X e : lc e -> lc <{ X@e }>
 | LCLit b : lc <{ lit b }>
 | LCSec e : lc e -> lc <{ s𝔹 e }>
-| LCIte l e0 e1 e2 : lc e0 -> lc e1 -> lc e2 -> lc <{ if{l} e0 then e1 else e2 }>
+| LCIte e0 e1 e2 : lc e0 -> lc e1 -> lc e2 -> lc <{ if e0 then e1 else e2 }>
 | LCProd l τ1 τ2 : lc τ1 -> lc τ2 -> lc <{ τ1 *{l} τ2 }>
 | LCPair l e1 e2 : lc e1 -> lc e2 -> lc <{ (e1, e2){l} }>
 | LCProj l b e : lc e -> lc <{ π{l}@b e }>
@@ -477,7 +413,6 @@ Inductive lc : expr -> Prop :=
 | LCInj l b τ e : lc τ -> lc e -> lc <{ inj{l}@b<τ> e }>
 | LCFold X e : lc e -> lc <{ fold<X> e }>
 | LCUnfold X e : lc e -> lc <{ unfold<X> e }>
-| LCTape e : lc e -> lc <{ tape e }>
 | LCMux e0 e1 e2 : lc e0 -> lc e1 -> lc e2 -> lc <{ mux e0 e1 e2 }>
 | LCBoxedLit b : lc <{ [b] }>
 (* Techincally this is not only locally closed, but more about
@@ -498,8 +433,9 @@ Notation "e ^ s" := (open s e) (in custom oadt at level 20).
 
 Notation "'{' x '↦' s '}' e" := (subst x s e)
                                   (in custom oadt at level 20, x constr).
+
 (* This notation is supposed to be applied to a typing context. *)
-Notation "{ x '↦' s }" := (lexpr_subst x s) (at level 20).
+Notation "{ x '↦' s }" := (subst x s) (at level 20).
 
 Notation "x # s" := (x ∉ stale s) (at level 40).
 
