theories/lang_oadt/typing.v
@@ -7,7 +7,7 @@ Implicit Types (b : bool) (x X y Y : atom) (L : aset).
 (** * Definitions *)
 
 (** ** Typing context (Γ) *)
-Notation tctx := (amap lexpr).
+Notation tctx := (amap expr).
 
 Section typing.
 
@@ -22,174 +22,123 @@ Context (Σ : gctx).
 Reserved Notation "e '⇛' e'" (at level 40).
 
 Inductive pared : expr -> expr -> Prop :=
-| RApp l τ e1 e2 e1' e2' L :
-    e1 ⇛ e1' ->
-    (forall x, x ∉ L -> <{ e2^x }> ⇛ <{ e2'^x }>) ->
-    lc τ ->
-    <{ (\:{l}τ => e2) e1 }> ⇛ <{ e2'^e1' }>
+| RApp τ e1 e2 e1' e2' L :
+  e1 ⇛ e1' ->
+  (forall x, x ∉ L -> <{ e2^x }> ⇛ <{ e2'^x }>) ->
+  lc τ ->
+  <{ (\:τ => e2) e1 }> ⇛ <{ e2'^e1' }>
 | RTApp X τ' τ e e' :
-    Σ !! X = Some (DOADT τ' τ) ->
-    e ⇛ e' ->
-    <{ X@e }> ⇛ <{ τ^e' }>
+  Σ !! X = Some (DOADT τ' τ) ->
+  e ⇛ e' ->
+  <{ X@e }> ⇛ <{ τ^e' }>
 | RLet e1 e2 e1' e2' L :
-    e1 ⇛ e1' ->
-    (forall x, x ∉ L -> <{ e2^x }> ⇛ <{ e2'^x }>) ->
-    <{ let e1 in e2 }> ⇛ <{ e2'^e1' }>
+  e1 ⇛ e1' ->
+  (forall x, x ∉ L -> <{ e2^x }> ⇛ <{ e2'^x }>) ->
+  <{ let e1 in e2 }> ⇛ <{ e2'^e1' }>
 | RFun x T e :
-    Σ !! x = Some (DFun T e) ->
-    <{ gvar x }> ⇛ <{ e }>
+  Σ !! x = Some (DFun T e) ->
+  <{ gvar x }> ⇛ <{ e }>
 | RProj l b e1 e2 e1' e2' :
-    e1 ⇛ e1' ->
-    e2 ⇛ e2' ->
-    <{ π{l}@b (e1, e2){l} }> ⇛ <{ ite b e1' e2' }>
-| RFold X X' e e' :
-    e ⇛ e' ->
-    <{ unfold<X> (fold<X'> e) }> ⇛ e'
+  e1 ⇛ e1' ->
+  e2 ⇛ e2' ->
+  <{ π{l}@b (e1, e2){l} }> ⇛ <{ ite b e1' e2' }>
+| RUnfold X X' e e' :
+  e ⇛ e' ->
+  <{ unfold<X> (fold<X'> e) }> ⇛ e'
 | RIte b e1 e2 e1' e2' :
-    e1 ⇛ e1' ->
-    e2 ⇛ e2' ->
-    <{ if b then e1 else e2 }> ⇛ <{ ite b e1' e2' }>
+  e1 ⇛ e1' ->
+  e2 ⇛ e2' ->
+  <{ if b then e1 else e2 }> ⇛ <{ ite b e1' e2' }>
 | RCase b τ e0 e1 e2 e0' e1' e2' L1 L2 :
-    e0 ⇛ e0' ->
-    (forall x, x ∉ L1 -> <{ e1^x }> ⇛ <{ e1'^x }>) ->
-    (forall x, x ∉ L2 -> <{ e2^x }> ⇛ <{ e2'^x }>) ->
-    lc τ ->
-    <{ case inj@b<τ> e0 of e1 | e2 }> ⇛ <{ ite b (e1'^e0') (e2'^e0') }>
+  e0 ⇛ e0' ->
+  (forall x, x ∉ L1 -> <{ e1^x }> ⇛ <{ e1'^x }>) ->
+  (forall x, x ∉ L2 -> <{ e2^x }> ⇛ <{ e2'^x }>) ->
+  lc τ ->
+  <{ case inj@b<τ> e0 of e1 | e2 }> ⇛ <{ ite b (e1'^e0') (e2'^e0') }>
 (* The rules for oblivous constructs are solely for proof convenience. They are
 not needed because they are not involved in type-level computation. *)
 | RMux b e1 e2 e1' e2' :
-    e1 ⇛ e1' ->
-    e2 ⇛ e2' ->
-    <{ mux [b] e1 e2 }> ⇛ <{ ite b e1' e2' }>
-(* This rule is needed for confluence. *)
-| ROIte b e1 e2 e1' e2' :
-    e1 ⇛ e1' ->
-    e2 ⇛ e2' ->
-    <{ ~if [b] then e1 else e2 }> ⇛ <{ ite b e1' e2' }>
+  e1 ⇛ e1' ->
+  e2 ⇛ e2' ->
+  <{ mux [b] e1 e2 }> ⇛ <{ ite b e1' e2' }>
 | ROCase b ω1 ω2 v v1 v2 e1 e2 e1' e2' L1 L2 :
-    oval v ->
-    ovalty v1 ω1 -> ovalty v2 ω2 ->
-    (forall x, x ∉ L1 -> <{ e1^x }> ⇛ <{ e1'^x }>) ->
-    (forall x, x ∉ L2 -> <{ e2^x }> ⇛ <{ e2'^x }>) ->
-    <{ ~case [inj@b<ω1 ~+ ω2> v] of e1 | e2 }> ⇛
-      <{ ~if [b] then (ite b (e1'^v) (e1'^v1)) else (ite b (e2'^v2) (e2'^v)) }>
-| RSec b :
-    <{ s𝔹 b }> ⇛ <{ [b] }>
+  oval v ->
+  ovalty v1 ω1 -> ovalty v2 ω2 ->
+  (forall x, x ∉ L1 -> <{ e1^x }> ⇛ <{ e1'^x }>) ->
+  (forall x, x ∉ L2 -> <{ e2^x }> ⇛ <{ e2'^x }>) ->
+  <{ ~case [inj@b<ω1 ~+ ω2> v] of e1 | e2 }> ⇛
+  <{ mux [b] (ite b (e1'^v) (e1'^v1)) (ite b (e2'^v2) (e2'^v)) }>
+| RSec b : <{ s𝔹 b }> ⇛ <{ [b] }>
 | ROInj b ω v :
-    otval ω -> oval v ->
-    <{ ~inj@b<ω> v }> ⇛ <{ [inj@b<ω> v] }>
-(* Unfortunately I have to spell out all the cases corresponding to [SOIte] for
-proof convenience. *)
-| ROIteApp b e1 e2 e e1' e2' e' :
-    e1 ⇛ e1' ->
-    e2 ⇛ e2' ->
-    e ⇛ e' ->
-    <{ (~if [b] then e1 else e2) e }> ⇛ <{ ~if [b] then e1' e' else e2' e' }>
-| ROIteSec b e1 e2 e1' e2' :
-    e1 ⇛ e1' ->
-    e2 ⇛ e2' ->
-    <{ s𝔹 (~if [b] then e1 else e2) }> ⇛ <{ ~if [b] then s𝔹 e1' else s𝔹 e2' }>
-| ROIteIte b e1 e2 e3 e4 e1' e2' e3' e4' :
-    e1 ⇛ e1' ->
-    e2 ⇛ e2' ->
-    e3 ⇛ e3' ->
-    e4 ⇛ e4' ->
-    <{ if (~if [b] then e1 else e2) then e3 else e4 }> ⇛
-      <{ ~if [b] then (if e1' then e3' else e4') else (if e2' then e3' else e4') }>
-| ROIteProj b b' e1 e2 e1' e2' :
-    e1 ⇛ e1' ->
-    e2 ⇛ e2' ->
-    <{ π@b' (~if [b] then e1 else e2) }> ⇛
-      <{ ~if [b] then π@b' e1' else π@b' e2' }>
-| ROIteCase b e1 e2 e3 e4 e1' e2' e3' e4' L1 L2 :
-    e1 ⇛ e1' ->
-    e2 ⇛ e2' ->
-    (forall x, x ∉ L1 -> <{ e3^x }> ⇛ <{ e3'^x }>) ->
-    (forall x, x ∉ L2 -> <{ e4^x }> ⇛ <{ e4'^x }>) ->
-    <{ case (~if [b] then e1 else e2) of e3 | e4 }> ⇛
-      <{ ~if [b] then (case e1' of e3' | e4') else (case e2' of e3' | e4') }>
-| ROIteUnfold X b e1 e2 e1' e2' :
-    e1 ⇛ e1' ->
-    e2 ⇛ e2' ->
-    <{ unfold<X> (~if [b] then e1 else e2) }> ⇛
-      <{ ~if [b] then unfold<X> e1' else unfold<X> e2' }>
-| RTapeOIte b e1 e2 e1' e2' :
-    e1 ⇛ e1' ->
-    e2 ⇛ e2' ->
-    <{ tape (~if [b] then e1 else e2) }> ⇛ <{ mux [b] (tape e1') (tape e2') }>
-| RTapeOVal v :
-    oval v ->
-    <{ tape v }> ⇛ v
+  otval ω -> oval v ->
+  <{ ~inj@b<ω> v }> ⇛ <{ [inj@b<ω> v] }>
 (* Congruence rules *)
-| RCgrPi l τ1 τ2 τ1' τ2' L :
-    τ1 ⇛ τ1' ->
-    (forall x, x ∉ L -> <{ τ2^x }> ⇛ <{ τ2'^x }>) ->
-    <{ Π:{l}τ1, τ2 }> ⇛ <{ Π:{l}τ1', τ2' }>
-| RCgrAbs l τ e τ' e' L :
-    τ ⇛ τ' ->
-    (forall x, x ∉ L -> <{ e^x }> ⇛ <{ e'^x }>) ->
-    <{ \:{l}τ => e }> ⇛ <{ \:{l}τ' => e' }>
+| RCgrPi τ1 τ2 τ1' τ2' L :
+  τ1 ⇛ τ1' ->
+  (forall x, x ∉ L -> <{ τ2^x }> ⇛ <{ τ2'^x }>) ->
+  <{ Π:τ1, τ2 }> ⇛ <{ Π:τ1', τ2' }>
+| RCgrAbs τ e τ' e' L :
+  τ ⇛ τ' ->
+  (forall x, x ∉ L -> <{ e^x }> ⇛ <{ e'^x }>) ->
+  <{ \:τ => e }> ⇛ <{ \:τ' => e' }>
 | RCgrApp e1 e2 e1' e2' :
-    e1 ⇛ e1' ->
-    e2 ⇛ e2' ->
-    <{ e1 e2 }> ⇛ <{ e1' e2' }>
+  e1 ⇛ e1' ->
+  e2 ⇛ e2' ->
+  <{ e1 e2 }> ⇛ <{ e1' e2' }>
 | RCgrTApp X e e' :
-    e ⇛ e' ->
-    <{ X@e }> ⇛ <{ X@e' }>
+  e ⇛ e' ->
+  <{ X@e }> ⇛ <{ X@e' }>
 | RCgrLet e1 e2 e1' e2' L :
-    e1 ⇛ e1' ->
-    (forall x, x ∉ L -> <{ e2^x }> ⇛ <{ e2'^x }>) ->
-    <{ let e1 in e2 }> ⇛ <{ let e1' in e2' }>
+  e1 ⇛ e1' ->
+  (forall x, x ∉ L -> <{ e2^x }> ⇛ <{ e2'^x }>) ->
+  <{ let e1 in e2 }> ⇛ <{ let e1' in e2' }>
 | RCgrSec e e' :
-    e ⇛ e' ->
-    <{ s𝔹 e }> ⇛ <{ s𝔹 e' }>
-| RCgrIte l e0 e1 e2 e0' e1' e2' :
-    e0 ⇛ e0' ->
-    e1 ⇛ e1' ->
-    e2 ⇛ e2' ->
-    <{ if{l} e0 then e1 else e2 }> ⇛ <{ if{l} e0' then e1' else e2' }>
+  e ⇛ e' ->
+  <{ s𝔹 e }> ⇛ <{ s𝔹 e' }>
+| RCgrIte e0 e1 e2 e0' e1' e2' :
+  e0 ⇛ e0' ->
+  e1 ⇛ e1' ->
+  e2 ⇛ e2' ->
+  <{ if e0 then e1 else e2 }> ⇛ <{ if e0' then e1' else e2' }>
 | RCgrProd l τ1 τ2 τ1' τ2' :
-    τ1 ⇛ τ1' ->
-    τ2 ⇛ τ2' ->
-    <{ τ1 *{l} τ2 }> ⇛ <{ τ1' *{l} τ2' }>
+  τ1 ⇛ τ1' ->
+  τ2 ⇛ τ2' ->
+  <{ τ1 *{l} τ2 }> ⇛ <{ τ1' *{l} τ2' }>
 | RCgrPair l e1 e2 e1' e2' :
-    e1 ⇛ e1' ->
-    e2 ⇛ e2' ->
-    <{ (e1, e2){l} }> ⇛ <{ (e1', e2'){l} }>
+  e1 ⇛ e1' ->
+  e2 ⇛ e2' ->
+  <{ (e1, e2){l} }> ⇛ <{ (e1', e2'){l} }>
 | RCgrProj l b e e' :
-    e ⇛ e' ->
-    <{ π{l}@b e }> ⇛ <{ π{l}@b e' }>
+  e ⇛ e' ->
+  <{ π{l}@b e }> ⇛ <{ π{l}@b e' }>
 | RCgrSum l τ1 τ2 τ1' τ2' :
-    τ1 ⇛ τ1' ->
-    τ2 ⇛ τ2' ->
-    <{ τ1 +{l} τ2 }> ⇛ <{ τ1' +{l} τ2' }>
+  τ1 ⇛ τ1' ->
+  τ2 ⇛ τ2' ->
+  <{ τ1 +{l} τ2 }> ⇛ <{ τ1' +{l} τ2' }>
 | RCgrInj l b τ e τ' e' :
-    e ⇛ e' ->
-    τ ⇛ τ' ->
-    <{ inj{l}@b<τ> e }> ⇛ <{ inj{l}@b<τ'> e' }>
+  e ⇛ e' ->
+  τ ⇛ τ' ->
+  <{ inj{l}@b<τ> e }> ⇛ <{ inj{l}@b<τ'> e' }>
 | RCgrCase l e0 e1 e2 e0' e1' e2' L1 L2 :
-    e0 ⇛ e0' ->
-    (forall x, x ∉ L1 -> <{ e1^x }> ⇛ <{ e1'^x }>) ->
-    (forall x, x ∉ L2 -> <{ e2^x }> ⇛ <{ e2'^x }>) ->
-    <{ case{l} e0 of e1 | e2 }> ⇛ <{ case{l} e0' of e1' | e2' }>
+  e0 ⇛ e0' ->
+  (forall x, x ∉ L1 -> <{ e1^x }> ⇛ <{ e1'^x }>) ->
+  (forall x, x ∉ L2 -> <{ e2^x }> ⇛ <{ e2'^x }>) ->
+  <{ case{l} e0 of e1 | e2 }> ⇛ <{ case{l} e0' of e1' | e2' }>
 | RCgrFold X e e' :
-    e ⇛ e' ->
-    <{ fold<X> e }> ⇛ <{ fold<X> e' }>
+  e ⇛ e' ->
+  <{ fold<X> e }> ⇛ <{ fold<X> e' }>
 | RCgrUnfold X e e' :
-    e ⇛ e' ->
-    <{ unfold<X> e }> ⇛ <{ unfold<X> e' }>
+  e ⇛ e' ->
+  <{ unfold<X> e }> ⇛ <{ unfold<X> e' }>
 | RCgrMux e0 e1 e2 e0' e1' e2' :
-    e0 ⇛ e0' ->
-    e1 ⇛ e1' ->
-    e2 ⇛ e2' ->
-    <{ mux e0 e1 e2 }> ⇛ <{ mux e0' e1' e2' }>
-| RCgrTape e e' :
-    e ⇛ e' ->
-    <{ tape e }> ⇛ <{ tape e' }>
+  e0 ⇛ e0' ->
+  e1 ⇛ e1' ->
+  e2 ⇛ e2' ->
+  <{ mux e0 e1 e2 }> ⇛ <{ mux e0' e1' e2' }>
 (* Reflexive rule *)
 | RRefl e :
-    lc e ->
-    e ⇛ e
+  lc e ->
+  e ⇛ e
 
 where "e1 '⇛' e2" := (pared e1 e2)
 .
@@ -205,13 +154,13 @@ most cases. *)
 Inductive pared_equiv : expr -> expr -> Prop :=
 | QRRefl e : e ≡ e
 | QRRedL e1 e1' e2 :
-    e1 ⇛ e1' ->
-    e1' ≡ e2 ->
-    e1 ≡ e2
+  e1 ⇛ e1' ->
+  e1' ≡ e2 ->
+  e1 ≡ e2
 | QRRedR e1 e2 e2' :
-    e2 ⇛ e2' ->
-    e1 ≡ e2' ->
-    e1 ≡ e2
+  e2 ⇛ e2' ->
+  e1 ≡ e2' ->
+  e1 ≡ e2
 
 where "e1 ≡ e2" := (pared_equiv e1 e2)
 .
@@ -222,186 +171,159 @@ Definition pared_equiv_join (e1 e2 : expr) : Prop :=
 
 (** ** Typing and kinding *)
 (** They are mutually defined. *)
-Reserved Notation "Γ '⊢' e ':{' l '}' τ" (at level 40,
-                                          e custom oadt at level 99,
-                                          l constr at level 99,
-                                          τ custom oadt at level 99).
+Reserved Notation "Γ '⊢' e ':' τ" (at level 40,
+    e custom oadt at level 99,
+    τ custom oadt at level 99).
 Reserved Notation "Γ '⊢' τ '::' κ" (at level 40,
-                                    τ custom oadt at level 99,
-                                    κ custom oadt at level 99).
+    τ custom oadt at level 99,
+    κ custom oadt at level 99).
 
-Inductive typing : tctx -> expr -> llabel -> expr -> Prop :=
-| TFVar Γ x l τ κ :
-    Γ !! x = Some (l, τ) ->
-    Γ ⊢ τ :: κ ->
-    Γ ⊢ fvar x :{l} τ
-| TGVar Γ x l τ e :
-    Σ !! x = Some (DFun (l, τ) e) ->
-    Γ ⊢ gvar x :{l} τ
-| TAbs Γ l1 l2 e τ1 τ2 κ L :
-    (forall x, x ∉ L -> <[x:=(l2, τ2)]>Γ ⊢ e^x :{l1} τ1^x) ->
-    Γ ⊢ τ2 :: κ ->
-    Γ ⊢ \:{l2}τ2 => e :{l1} (Π:{l2}τ2, τ1)
-| TLet Γ l1 l2 e1 e2 τ1 τ2 L :
-    Γ ⊢ e1 :{l1} τ1 ->
-    (forall x, x ∉ L -> <[x:=(l1, τ1)]>Γ ⊢ e2^x :{l2} τ2^x) ->
-    Γ ⊢ let e1 in e2 :{l2} τ2^e1
-| TApp Γ l1 l2 e1 e2 τ1 τ2 :
-    Γ ⊢ e1 :{l1} (Π:{l2}τ2, τ1) ->
-    Γ ⊢ e2 :{l2} τ2 ->
-    Γ ⊢ e1 e2 :{l1} τ1^e2
-| TUnit Γ : Γ ⊢ () :{⊥} 𝟙
-| TLit Γ b : Γ ⊢ lit b :{⊥} 𝔹
-| TSec Γ l e :
-    Γ ⊢ e :{l} 𝔹 ->
-    Γ ⊢ s𝔹 e :{l} ~𝔹
-| TIte Γ l1 l2 l e0 e1 e2 τ κ :
-    Γ ⊢ e0 :{⊥} 𝔹 ->
-    Γ ⊢ e1 :{l1} τ^(lit true) ->
-    Γ ⊢ e2 :{l2} τ^(lit false) ->
-    Γ ⊢ τ^e0 :: κ ->
-    l = l1 ⊔ l2 ->
-    Γ ⊢ if e0 then e1 else e2 :{l} τ^e0
-| TIteNoDep Γ l0 l1 l2 l e0 e1 e2 τ :
-    Γ ⊢ e0 :{l0} 𝔹 ->
-    Γ ⊢ e1 :{l1} τ ->
-    Γ ⊢ e2 :{l2} τ ->
-    l = l0 ⊔ l1 ⊔ l2 ->
-    Γ ⊢ if e0 then e1 else e2 :{l} τ
-| TOIte Γ l1 l2 e0 e1 e2 τ κ :
-    Γ ⊢ e0 :{⊥} ~𝔹 ->
-    Γ ⊢ e1 :{l1} τ ->
-    Γ ⊢ e2 :{l2} τ ->
-    Γ ⊢ τ :: κ ->
-    Γ ⊢ ~if e0 then e1 else e2 :{⊤} τ
-| TInj Γ l b e τ1 τ2 κ :
-    Γ ⊢ e :{l} ite b τ1 τ2 ->
-    Γ ⊢ τ1 + τ2 :: κ ->
-    Γ ⊢ inj@b<τ1 + τ2> e :{l} τ1 + τ2
+Inductive typing : tctx -> expr -> expr -> Prop :=
+| TFVar Γ x τ κ :
+  Γ !! x = Some τ ->
+  Γ ⊢ τ :: κ ->
+  Γ ⊢ fvar x : τ
+| TGVar Γ x τ e :
+  Σ !! x = Some (DFun τ e) ->
+  Γ ⊢ gvar x : τ
+| TAbs Γ e τ1 τ2 κ L :
+  (forall x, x ∉ L -> <[x:=τ2]>Γ ⊢ e^x : τ1^x) ->
+  Γ ⊢ τ2 :: κ ->
+  Γ ⊢ \:τ2 => e : (Π:τ2, τ1)
+| TLet Γ e1 e2 τ1 τ2 L :
+  Γ ⊢ e1 : τ1 ->
+  (forall x, x ∉ L -> <[x:=τ1]>Γ ⊢ e2^x : τ2^x) ->
+  Γ ⊢ let e1 in e2 : τ2^e1
+| TApp Γ e1 e2 τ1 τ2 :
+  Γ ⊢ e1 : (Π:τ2, τ1) ->
+  Γ ⊢ e2 : τ2 ->
+  Γ ⊢ e1 e2 : τ1^e2
+| TUnit Γ : Γ ⊢ () : 𝟙
+| TLit Γ b : Γ ⊢ lit b : 𝔹
+| TSec Γ e :
+  Γ ⊢ e : 𝔹 ->
+  Γ ⊢ s𝔹 e : ~𝔹
+| TIte Γ e0 e1 e2 τ κ :
+  Γ ⊢ e0 : 𝔹 ->
+  Γ ⊢ e1 : τ^(lit true) ->
+  Γ ⊢ e2 : τ^(lit false) ->
+  Γ ⊢ τ^e0 :: κ ->
+  Γ ⊢ if e0 then e1 else e2 : τ^e0
+| TInj Γ b e τ1 τ2 κ :
+  Γ ⊢ e : ite b τ1 τ2 ->
+  Γ ⊢ τ1 + τ2 :: κ ->
+  Γ ⊢ inj@b<τ1 + τ2> e : τ1 + τ2
 | TOInj Γ b e τ1 τ2 :
-    Γ ⊢ e :{⊥} ite b τ1 τ2 ->
-    Γ ⊢ τ1 ~+ τ2 :: *@O ->
-    Γ ⊢ ~inj@b<τ1 ~+ τ2> e :{⊥} τ1 ~+ τ2
-| TCase Γ l1 l2 l e0 e1 e2 τ1 τ2 τ κ L1 L2 :
-    Γ ⊢ e0 :{⊥} τ1 + τ2 ->
-    (forall x, x ∉ L1 -> <[x:=(⊥, τ1)]>Γ ⊢ e1^x :{l1} τ^(inl<τ1 + τ2> x)) ->
-    (forall x, x ∉ L2 -> <[x:=(⊥, τ2)]>Γ ⊢ e2^x :{l2} τ^(inr<τ1 + τ2> x)) ->
-    Γ ⊢ τ^e0 :: κ ->
-    l = l1 ⊔ l2 ->
-    Γ ⊢ case e0 of e1 | e2 :{l} τ^e0
-| TCaseNoDep Γ l0 l1 l2 l e0 e1 e2 τ1 τ2 τ κ L1 L2 :
-    Γ ⊢ e0 :{l0} τ1 + τ2 ->
-    (forall x, x ∉ L1 -> <[x:=(l0, τ1)]>Γ ⊢ e1^x :{l1} τ) ->
-    (forall x, x ∉ L2 -> <[x:=(l0, τ2)]>Γ ⊢ e2^x :{l2} τ) ->
-    Γ ⊢ τ :: κ ->
-    l = l0 ⊔ l1 ⊔ l2 ->
-    Γ ⊢ case e0 of e1 | e2 :{l} τ
-| TOCase Γ l1 l2 e0 e1 e2 τ1 τ2 τ κ L1 L2 :
-    Γ ⊢ e0 :{⊥} τ1 ~+ τ2 ->
-    (forall x, x ∉ L1 -> <[x:=(⊥, τ1)]>Γ ⊢ e1^x :{l1} τ) ->
-    (forall x, x ∉ L2 -> <[x:=(⊥, τ2)]>Γ ⊢ e2^x :{l2} τ) ->
-    Γ ⊢ τ :: κ ->
-    Γ ⊢ ~case e0 of e1 | e2 :{⊤} τ
-| TPair Γ l1 l2 l e1 e2 τ1 τ2 :
-    Γ ⊢ e1 :{l1} τ1 ->
-    Γ ⊢ e2 :{l2} τ2 ->
-    l = l1 ⊔ l2 ->
-    Γ ⊢ (e1, e2) :{l} τ1 * τ2
+  Γ ⊢ e : ite b τ1 τ2 ->
+  Γ ⊢ τ1 ~+ τ2 :: *@O ->
+  Γ ⊢ ~inj@b<τ1 ~+ τ2> e : τ1 ~+ τ2
+| TCase Γ e0 e1 e2 τ1 τ2 τ κ L1 L2 :
+  Γ ⊢ e0 : τ1 + τ2 ->
+  (forall x, x ∉ L1 -> <[x:=τ1]>Γ ⊢ e1^x : τ^(inl<τ1 + τ2> x)) ->
+  (forall x, x ∉ L2 -> <[x:=τ2]>Γ ⊢ e2^x : τ^(inr<τ1 + τ2> x)) ->
+  Γ ⊢ τ^e0 :: κ ->
+  Γ ⊢ case e0 of e1 | e2 : τ^e0
+| TOCase Γ e0 e1 e2 τ1 τ2 τ L1 L2 :
+  Γ ⊢ e0 : τ1 ~+ τ2 ->
+  (forall x, x ∉ L1 -> <[x:=τ1]>Γ ⊢ e1^x : τ) ->
+  (forall x, x ∉ L2 -> <[x:=τ2]>Γ ⊢ e2^x : τ) ->
+  Γ ⊢ τ :: *@O ->
+  Γ ⊢ ~case e0 of e1 | e2 : τ
+| TPair Γ e1 e2 τ1 τ2 :
+  Γ ⊢ e1 : τ1 ->
+  Γ ⊢ e2 : τ2 ->
+  Γ ⊢ (e1, e2) : τ1 * τ2
 | TOPair Γ e1 e2 τ1 τ2 :
-    Γ ⊢ e1 :{⊥} τ1 ->
-    Γ ⊢ e2 :{⊥} τ2 ->
-    Γ ⊢ τ1 :: *@O ->
-    Γ ⊢ τ2 :: *@O ->
-    Γ ⊢ ~(e1, e2) :{⊥} τ1 ~* τ2
-| TProj Γ l b e τ1 τ2 :
-    Γ ⊢ e :{l} τ1 * τ2 ->
-    Γ ⊢ π@b e :{l} ite b τ1 τ2
+  Γ ⊢ e1 : τ1 ->
+  Γ ⊢ e2 : τ2 ->
+  Γ ⊢ τ1 :: *@O ->
+  Γ ⊢ τ2 :: *@O ->
+  Γ ⊢ ~(e1, e2) : τ1 ~* τ2
+| TProj Γ b e τ1 τ2 :
+  Γ ⊢ e : τ1 * τ2 ->
+  Γ ⊢ π@b e : ite b τ1 τ2
 | TOProj Γ b e τ1 τ2 :
-    Γ ⊢ e :{⊥} τ1 ~* τ2 ->
-    Γ ⊢ ~π@b e :{⊥} ite b τ1 τ2
-| TFold Γ l X e τ :
-    Σ !! X = Some (DADT τ) ->
-    Γ ⊢ e :{l} τ ->
-    Γ ⊢ fold<X> e :{l} gvar X
-| TUnfold Γ l X e τ :
-    Σ !! X = Some (DADT τ) ->
-    Γ ⊢ e :{l} gvar X ->
-    Γ ⊢ unfold<X> e :{l} τ
+  Γ ⊢ e : τ1 ~* τ2 ->
+  Γ ⊢ ~π@b e : ite b τ1 τ2
+| TFold Γ X e τ :
+  Σ !! X = Some (DADT τ) ->
+  Γ ⊢ e : τ ->
+  Γ ⊢ fold<X> e : gvar X
+| TUnfold Γ X e τ :
+  Σ !! X = Some (DADT τ) ->
+  Γ ⊢ e : gvar X ->
+  Γ ⊢ unfold<X> e : τ
 | TMux Γ e0 e1 e2 τ :
-    Γ ⊢ e0 :{⊥} ~𝔹 ->
-    Γ ⊢ e1 :{⊥} τ ->
-    Γ ⊢ e2 :{⊥} τ ->
-    Γ ⊢ τ :: *@O ->
-    Γ ⊢ mux e0 e1 e2 :{⊥} τ
-| TTape Γ l e τ :
-    Γ ⊢ e :{l} τ ->
-    Γ ⊢ τ :: *@O ->
-    Γ ⊢ tape e :{⊥} τ
+  Γ ⊢ e0 : ~𝔹 ->
+  Γ ⊢ e1 : τ ->
+  Γ ⊢ e2 : τ ->
+  Γ ⊢ τ :: *@O ->
+  Γ ⊢ mux e0 e1 e2 : τ
 (* Typing for runtime expressions is for metatheories. These expressions do not
 appear in source programs. Plus, it is not possible to type them at runtime
 since they are "encrypted" values. *)
-| TBoxedLit Γ b : Γ ⊢ [b] :{⊥} ~𝔹
+| TBoxedLit Γ b : Γ ⊢ [b] : ~𝔹
 | TBoxedInj Γ b v ω :
-    ovalty <{ [inj@b<ω> v] }> ω ->
-    Γ ⊢ [inj@b<ω> v] :{⊥} ω
+  ovalty <{ [inj@b<ω> v] }> ω ->
+  Γ ⊢ [inj@b<ω> v] : ω
 (* Type conversion *)
-| TConv Γ l l' e τ τ' κ :
-    Γ ⊢ e :{l'} τ' ->
-    τ' ≡ τ ->
-    Γ ⊢ τ :: κ ->
-    l' ⊑ l ->
-    Γ ⊢ e :{l} τ
+| TConv Γ e τ τ' κ :
+  Γ ⊢ e : τ' ->
+  τ' ≡ τ ->
+  Γ ⊢ τ :: κ ->
+  Γ ⊢ e : τ
 
 with kinding : tctx -> expr -> kind -> Prop :=
 | KGVar Γ X τ :
-    Σ !! X = Some (DADT τ) ->
-    Γ ⊢ gvar X :: *@P
+  Σ !! X = Some (DADT τ) ->
+  Γ ⊢ gvar X :: *@P
 | KUnit Γ : Γ ⊢ 𝟙 :: *@A
-| KBool Γ l : Γ ⊢ 𝔹{l} :: ite l *@O *@P
-| KPi Γ l τ1 τ2 κ1 κ2 L :
-    (forall x, x ∉ L -> <[x:=(l, τ1)]>Γ ⊢ τ2^x :: κ2) ->
-    Γ ⊢ τ1 :: κ1 ->
-    Γ ⊢ (Π:{l}τ1, τ2) :: *@M
+| KBool Γ : Γ ⊢ 𝔹 :: *@P
+| KOBool Γ : Γ ⊢ ~𝔹 :: *@O
+| KPi Γ τ1 τ2 κ1 κ2 L :
+  (forall x, x ∉ L -> <[x:=τ1]>Γ ⊢ τ2^x :: κ2) ->
+  Γ ⊢ τ1 :: κ1 ->
+  Γ ⊢ (Π:τ1, τ2) :: *@M
 | KApp Γ e' e τ X :
-    Σ !! X = Some (DOADT τ e') ->
-    Γ ⊢ e :{⊥} τ ->
-    Γ ⊢ X@e :: *@O
+  Σ !! X = Some (DOADT τ e') ->
+  Γ ⊢ e : τ ->
+  Γ ⊢ X@e :: *@O
 | KProd Γ τ1 τ2 κ :
-    Γ ⊢ τ1 :: κ ->
-    Γ ⊢ τ2 :: κ ->
-    Γ ⊢ τ1 * τ2 :: (κ ⊔ *@P)
+  Γ ⊢ τ1 :: κ ->
+  Γ ⊢ τ2 :: κ ->
+  Γ ⊢ τ1 * τ2 :: (κ ⊔ *@P)
 | KOProd Γ τ1 τ2 :
-    Γ ⊢ τ1 :: *@O ->
-    Γ ⊢ τ2 :: *@O ->
-    Γ ⊢ τ1 ~* τ2 :: *@O
+  Γ ⊢ τ1 :: *@O ->
+  Γ ⊢ τ2 :: *@O ->
+  Γ ⊢ τ1 ~* τ2 :: *@O
 | KSum Γ τ1 τ2 κ :
-    Γ ⊢ τ1 :: κ ->
-    Γ ⊢ τ2 :: κ ->
-    Γ ⊢ τ1 + τ2 :: (κ ⊔ *@P)
+  Γ ⊢ τ1 :: κ ->
+  Γ ⊢ τ2 :: κ ->
+  Γ ⊢ τ1 + τ2 :: (κ ⊔ *@P)
 | KOSum Γ τ1 τ2 :
-    Γ ⊢ τ1 :: *@O ->
-    Γ ⊢ τ2 :: *@O ->
-    Γ ⊢ τ1 ~+ τ2 :: *@O
+  Γ ⊢ τ1 :: *@O ->
+  Γ ⊢ τ2 :: *@O ->
+  Γ ⊢ τ1 ~+ τ2 :: *@O
 | KIte Γ e0 τ1 τ2 :
-    Γ ⊢ e0 :{⊥} 𝔹 ->
-    Γ ⊢ τ1 :: *@O ->
-    Γ ⊢ τ2 :: *@O ->
-    Γ ⊢ if e0 then τ1 else τ2 :: *@O
+  Γ ⊢ e0 : 𝔹 ->
+  Γ ⊢ τ1 :: *@O ->
+  Γ ⊢ τ2 :: *@O ->
+  Γ ⊢ if e0 then τ1 else τ2 :: *@O
 | KCase Γ e0 τ1 τ2 τ1' τ2' L1 L2 :
-    Γ ⊢ e0 :{⊥} τ1' + τ2' ->
-    (forall x, x ∉ L1 -> <[x:=(⊥, τ1')]>Γ ⊢ τ1^x :: *@O) ->
-    (forall x, x ∉ L2 -> <[x:=(⊥, τ2')]>Γ ⊢ τ2^x :: *@O) ->
-    Γ ⊢ case e0 of τ1 | τ2 :: *@O
+  Γ ⊢ e0 : τ1' + τ2' ->
+  (forall x, x ∉ L1 -> <[x:=τ1']>Γ ⊢ τ1^x :: *@O) ->
+  (forall x, x ∉ L2 -> <[x:=τ2']>Γ ⊢ τ2^x :: *@O) ->
+  Γ ⊢ case e0 of τ1 | τ2 :: *@O
 | KLet Γ e τ τ' L :
-    Γ ⊢ e :{⊥} τ' ->
-    (forall x, x ∉ L -> <[x:=(⊥, τ')]>Γ ⊢ τ^x :: *@O) ->
-    Γ ⊢ let e in τ :: *@O
+  Γ ⊢ e : τ' ->
+  (forall x, x ∉ L -> <[x:=τ']>Γ ⊢ τ^x :: *@O) ->
+  Γ ⊢ let e in τ :: *@O
 | KSub Γ τ κ κ' :
-    Γ ⊢ τ :: κ' ->
-    κ' ⊑ κ ->
-    Γ ⊢ τ :: κ
+  Γ ⊢ τ :: κ' ->
+  κ' ⊑ κ ->
+  Γ ⊢ τ :: κ
 
-where "Γ '⊢' e ':{' l '}' τ" := (typing Γ e l τ)
+where "Γ '⊢' e ':' τ" := (typing Γ e τ)
   and "Γ '⊢' τ '::' κ" := (kinding Γ τ κ)
 .
 
@@ -409,41 +331,40 @@ End fix_gctx.
 
 (** Better induction principle. *)
 Scheme typing_kinding_ind := Minimality for typing Sort Prop
-  with kinding_typing_ind := Minimality for kinding Sort Prop.
+    with kinding_typing_ind := Minimality for kinding Sort Prop.
 Combined Scheme typing_kinding_mutind
-         from typing_kinding_ind, kinding_typing_ind.
+  from typing_kinding_ind, kinding_typing_ind.
 
 Notation "Σ '⊢' e '≡' e'" := (pared_equiv Σ e e')
                                (at level 40,
-                                e custom oadt at level 99,
-                                e' custom oadt at level 99).
-Notation "Σ ; Γ '⊢' e ':{' l '}' τ" := (typing Σ Γ e l τ)
-                                         (at level 40,
-                                           Γ constr at next level,
-                                           e custom oadt at level 99,
-                                           τ custom oadt at level 99,
-                                           format "Σ ;  Γ  '⊢'  e  ':{' l '}'  τ").
+                                 e custom oadt at level 99,
+                                 e' custom oadt at level 99).
+Notation "Σ ; Γ '⊢' e ':' τ" := (typing Σ Γ e τ)
+                                  (at level 40,
+                                    Γ constr at next level,
+                                    e custom oadt at level 99,
+                                    τ custom oadt at level 99).
 Notation "Σ ; Γ '⊢' τ '::' κ" := (kinding Σ Γ τ κ)
                                    (at level 40,
-                                    Γ constr at next level,
-                                    τ custom oadt at level 99,
-                                    κ custom oadt at level 99).
+                                     Γ constr at next level,
+                                     τ custom oadt at level 99,
+                                     κ custom oadt at level 99).
 
 (** ** Global definitions typing *)
 Reserved Notation "Σ '⊢₁' D" (at level 40).
 
 Inductive gdef_typing : gctx -> gdef -> Prop :=
 | DTADT Σ τ :
-    Σ; ∅ ⊢ τ :: *@P ->
-    Σ ⊢₁ (DADT τ)
+  Σ; ∅ ⊢ τ :: *@P ->
+  Σ ⊢₁ (DADT τ)
 | DTOADT Σ τ e L :
-    Σ; ∅ ⊢ τ :: *@P ->
-    (forall x, x ∉ L -> Σ; ({[x:=(⊥, τ)]}) ⊢ e^x :: *@O) ->
-    Σ ⊢₁ (DOADT τ e)
-| DTFun Σ l τ e κ :
-    Σ; ∅ ⊢ τ :: κ ->
-    Σ; ∅ ⊢ e :{l} τ ->
-    Σ ⊢₁ (DFun (l, τ) e)
+  Σ; ∅ ⊢ τ :: *@P ->
+  (forall x, x ∉ L -> Σ; ({[x:=τ]}) ⊢ e^x :: *@O) ->
+  Σ ⊢₁ (DOADT τ e)
+| DTFun Σ τ e κ :
+  Σ; ∅ ⊢ τ :: κ ->
+  Σ; ∅ ⊢ e : τ ->
+  Σ ⊢₁ (DFun τ e)
 
 where "Σ '⊢₁' D" := (gdef_typing Σ D)
 .
@@ -454,7 +375,7 @@ Definition gctx_typing (Σ : gctx) : Prop :=
 (** ** Program typing *)
 (** The top level expression should not contain potential leaks. *)
 Definition program_typing (Σ : gctx) (e : expr) (τ : expr) :=
-  gctx_typing Σ /\ Σ; ∅ ⊢ e :{⊥} τ.
+  gctx_typing Σ /\ Σ; ∅ ⊢ e : τ.
 
 (** ** Well-formedness of global context *)
 (** Equivalent to [gctx_typing]. Essentially saying all definitions in [Σ] are
@@ -465,13 +386,13 @@ Definition gctx_wf (Σ : gctx) :=
   map_Forall (fun _ D =>
                 match D with
                 | DADT τ =>
-                  Σ; ∅ ⊢ τ :: *@P
+                    Σ; ∅ ⊢ τ :: *@P
                 | DOADT τ e =>
-                  Σ; ∅ ⊢ τ :: *@P /\
-                  exists L, forall x, x ∉ L -> Σ; ({[x:=(⊥, τ)]}) ⊢ e^x :: *@O
-                | DFun (l, τ) e =>
-                  Σ; ∅ ⊢ e :{l} τ /\
-                  exists κ, Σ; ∅ ⊢ τ :: κ
+                    Σ; ∅ ⊢ τ :: *@P /\
+                    exists L, forall x, x ∉ L -> Σ; ({[x:=τ]}) ⊢ e^x :: *@O
+                | DFun τ e =>
+                    Σ; ∅ ⊢ e : τ /\
+                    exists κ, Σ; ∅ ⊢ τ :: κ
                 end) Σ.
 
 End typing.
@@ -492,25 +413,18 @@ Notation "Σ '⊢' e '⇛*' e'" := (rtc (pared Σ) e e')
                                   e' custom oadt at level 99).
 Notation "Σ '⊢' e '≡' e'" := (pared_equiv Σ e e')
                                (at level 40,
-                                e custom oadt at level 99,
-                                e' custom oadt at level 99).
-Notation "Σ ; Γ '⊢' e ':{' l '}' τ" := (typing Σ Γ e l τ)
-                                         (at level 40,
-                                           Γ constr at next level,
-                                           e custom oadt at level 99,
-                                           τ custom oadt at level 99,
-                                           format "Σ ;  Γ  '⊢'  e  ':{' l '}'  τ").
-Notation "Σ ; Γ '⊢' e ':' τ" := (typing Σ Γ e _ τ)
-                                         (at level 40,
-                                           Γ constr at next level,
-                                           e custom oadt at level 99,
-                                           τ custom oadt at level 99,
-                                           only parsing).
+                                 e custom oadt at level 99,
+                                 e' custom oadt at level 99).
+Notation "Σ ; Γ '⊢' e ':' τ" := (typing Σ Γ e τ)
+                                  (at level 40,
+                                    Γ constr at next level,
+                                    e custom oadt at level 99,
+                                    τ custom oadt at level 99).
 Notation "Σ ; Γ '⊢' τ '::' κ" := (kinding Σ Γ τ κ)
                                    (at level 40,
-                                    Γ constr at next level,
-                                    τ custom oadt at level 99,
-                                    κ custom oadt at level 99).
+                                     Γ constr at next level,
+                                     τ custom oadt at level 99,
+                                     κ custom oadt at level 99).
 
 Notation "Σ '⊢₁' D" := (gdef_typing Σ D) (at level 40).
 
@@ -521,17 +435,10 @@ Notation "Σ ; e '▷' τ" := (program_typing Σ e τ)
 Notation "e '⇛' e'" := (pared _ e e') (at level 40).
 Notation "e '⇛*' e'" := (rtc (pared _) e e') (at level 40).
 
-Notation "Γ '⊢' e ':{' l '}' τ" := (typing _ Γ e l τ)
-                                     (at level 40,
-                                       e custom oadt at level 99,
-                                       l constr at level 99,
-                                       τ custom oadt at level 99,
-                                       format "Γ  '⊢'  e  ':{' l '}'  τ").
-Notation "Γ '⊢' e ':' τ" := (typing _ Γ e _ τ)
+Notation "Γ '⊢' e ':' τ" := (typing _ Γ e τ)
                               (at level 40,
                                 e custom oadt at level 99,
-                                τ custom oadt at level 99,
-                                only parsing).
+                                τ custom oadt at level 99).
 Notation "Γ '⊢' τ '::' κ" := (kinding _ Γ τ κ)
                                (at level 40,
                                  τ custom oadt at level 99,
