theories/lang_oadt/progress.v
@@ -45,34 +45,21 @@ Proof.
     eauto using pared_obliv_preservation_inv, pared_kinding_preservation.
 Qed.
 
-Lemma wval_woval Γ v l τ :
-  Γ ⊢ v :{l} τ ->
+Lemma val_oval Γ v τ :
+  Γ ⊢ v : τ ->
   Γ ⊢ τ :: *@O ->
-  wval v ->
-  woval v.
+  val v ->
+  oval v.
 Proof.
-  induction 1; intros; try wval_inv; try oval_inv;
+  induction 1; intros; try val_inv; try oval_inv;
     kind_inv; simplify_eq;
-      try hauto lq: on ctrs: woval, oval; try easy.
+      try hauto lq: on ctrs: oval; try easy.
 
   (* TConv *)
   apply_regularity.
   auto_apply; eauto.
   eapply pared_equiv_obliv_preservation; eauto.
   equiv_naive_solver.
-Qed.
-
-Lemma val_oval Γ v l τ :
-  Γ ⊢ v :{l} τ ->
-  Γ ⊢ τ :: *@O ->
-  val v ->
-  oval v.
-Proof.
-  intros Ht Hk Hv.
-  pose proof Hv.
-  apply val_wval in Hv.
-  eapply wval_woval in Hv; eauto.
-  sinvert Hv; eauto. val_inv. oval_inv.
 Qed.
 
 (** * Canonical forms *)
@@ -86,65 +73,65 @@ Ltac canonical_form_solver :=
   simplify_eq;
   eauto 10.
 
-Lemma canonical_form_unit Γ l e :
+Lemma canonical_form_unit Γ e :
   val e ->
-  Γ ⊢ e :{l} 𝟙 ->
+  Γ ⊢ e : 𝟙 ->
   e = <{ () }>.
 Proof.
   canonical_form_solver.
 Qed.
 
-Lemma canonical_form_abs Γ l1 l2 e τ2 τ1 :
+Lemma canonical_form_abs Γ e τ2 τ1 :
   val e ->
-  Γ ⊢ e :{l1} Π:{l2}τ2, τ1 ->
-  exists e' τ, e = <{ \:{l2}τ => e' }>.
+  Γ ⊢ e : Π:τ2, τ1 ->
+  exists e' τ, e = <{ \:τ => e' }>.
 Proof.
   canonical_form_solver.
 Qed.
 
-Lemma canonical_form_bool Γ l e :
+Lemma canonical_form_bool Γ e :
   val e ->
-  Γ ⊢ e :{l} 𝔹 ->
+  Γ ⊢ e : 𝔹 ->
   exists b, e = <{ b }>.
 Proof.
   canonical_form_solver.
 Qed.
 
-Lemma canonical_form_obool Γ l e :
+Lemma canonical_form_obool Γ e :
   val e ->
-  Γ ⊢ e :{l} ~𝔹 ->
+  Γ ⊢ e : ~𝔹 ->
   exists b, e = <{ [b] }>.
 Proof.
   canonical_form_solver.
 Qed.
 
-Lemma canonical_form_prod Γ l e τ1 τ2 :
+Lemma canonical_form_prod Γ e τ1 τ2 :
   val e ->
-  Γ ⊢ e :{l} τ1 * τ2 ->
+  Γ ⊢ e : τ1 * τ2 ->
   exists v1 v2, val v1 /\ val v2 /\ e = <{ (v1, v2) }>.
 Proof.
   canonical_form_solver.
 Qed.
 
-Lemma canonical_form_oprod Γ l e τ1 τ2 :
+Lemma canonical_form_oprod Γ e τ1 τ2 :
   val e ->
-  Γ ⊢ e :{l} τ1 ~* τ2 ->
+  Γ ⊢ e : τ1 ~* τ2 ->
   exists v1 v2, oval v1 /\ oval v2 /\ e = <{ ~(v1, v2) }>.
 Proof.
   canonical_form_solver.
 Qed.
 
-Lemma canonical_form_sum Γ l e τ1 τ2 :
+Lemma canonical_form_sum Γ e τ1 τ2 :
   val e ->
-  Γ ⊢ e :{l} τ1 + τ2 ->
+  Γ ⊢ e : τ1 + τ2 ->
   exists b v τ, val v /\ e = <{ inj@b<τ> v }>.
 Proof.
   canonical_form_solver.
 Qed.
 
-Lemma canonical_form_osum Γ l e τ1 τ2 :
+Lemma canonical_form_osum Γ e τ1 τ2 :
   val e ->
-  Γ ⊢ e :{l} τ1 ~+ τ2 ->
+  Γ ⊢ e : τ1 ~+ τ2 ->
   exists b v ω1 ω2, oval v /\ otval ω1 /\ otval ω2 /\
                e = <{ [inj@b<ω1 ~+ ω2> v] }>.
 Proof.
@@ -157,66 +144,10 @@ Qed.
 
 (** Though it seems we should have a condition of [X] being an (public) ADT, this
 condition is not needed since it is implied by the typing judgment. *)
-Lemma canonical_form_fold Γ l e X :
+Lemma canonical_form_fold Γ e X :
   val e ->
-  Γ ⊢ e :{l} gvar X ->
+  Γ ⊢ e : gvar X ->
   exists v X', val v /\ e = <{ fold<X'> v }>.
-Proof.
-  inversion 1; canonical_form_solver.
-Qed.
-
-(** * Canonical forms for weak values *)
-
-Lemma canonical_form_weak_unit Γ l e :
-  wval e ->
-  Γ ⊢ e :{l} 𝟙 ->
-  e = <{ () }> \/
-  (exists b v1 v2, wval v1 /\ wval v2 /\ e = <{ ~if [b] then v1 else v2 }>).
-Proof.
-  canonical_form_solver.
-Qed.
-
-Lemma canonical_form_weak_abs Γ l1 l2 e τ2 τ1 :
-  wval e ->
-  Γ ⊢ e :{l1} Π:{l2}τ2, τ1 ->
-  (exists e' τ, e = <{ \:{l2}τ => e' }>) \/
-  (exists b v1 v2, wval v1 /\ wval v2 /\ e = <{ ~if [b] then v1 else v2 }>).
-Proof.
-  canonical_form_solver.
-Qed.
-
-Lemma canonical_form_weak_bool Γ l e :
-  wval e ->
-  Γ ⊢ e :{l} 𝔹 ->
-  (exists b, e = <{ b }>) \/
-  (exists b v1 v2, wval v1 /\ wval v2 /\ e = <{ ~if [b] then v1 else v2 }>).
-Proof.
-  canonical_form_solver.
-Qed.
-
-Lemma canonical_form_weak_prod Γ l e τ1 τ2 :
-  wval e ->
-  Γ ⊢ e :{l} τ1 * τ2 ->
-  (exists v1 v2, wval v1 /\ wval v2 /\ e = <{ (v1, v2) }>) \/
-  (exists b v1 v2, wval v1 /\ wval v2 /\ e = <{ ~if [b] then v1 else v2 }>).
-Proof.
-  canonical_form_solver.
-Qed.
-
-Lemma canonical_form_weak_sum Γ l e τ1 τ2 :
-  wval e ->
-  Γ ⊢ e :{l} τ1 + τ2 ->
-  (exists b v τ, wval v /\ e = <{ inj@b<τ> v }>) \/
-  (exists b v1 v2, wval v1 /\ wval v2 /\ e = <{ ~if [b] then v1 else v2 }>).
-Proof.
-  canonical_form_solver.
-Qed.
-
-Lemma canonical_form_weak_fold Γ l e X :
-  wval e ->
-  Γ ⊢ e :{l} gvar X ->
-  (exists v X', wval v /\ e = <{ fold<X'> v }>) \/
-  (exists b v1 v2, wval v1 /\ wval v2 /\ e = <{ ~if [b] then v1 else v2 }>).
 Proof.
   inversion 1; canonical_form_solver.
 Qed.
@@ -226,38 +157,22 @@ End fix_gctx.
 Ltac apply_canonical_form_lem τ :=
   lazymatch τ with
   | <{ 𝟙 }> => canonical_form_unit
+  | <{ 𝔹 }> => canonical_form_bool
   | <{ ~𝔹 }> => canonical_form_obool
+  | <{ _ * _ }> => canonical_form_prod
   | <{ _ ~* _ }> => canonical_form_oprod
+  | <{ _ + _ }> => canonical_form_sum
   | <{ _ ~+ _ }> => canonical_form_osum
+  | <{ Π:_, _ }> => canonical_form_abs
+  | <{ gvar _ }> => canonical_form_fold
   end.
 
 Ltac apply_canonical_form :=
   match goal with
-  | H : val ?e, H' : _; _ ⊢ ?e :{_} ?τ |- _ =>
+  | H : val ?e, H' : _; _ ⊢ ?e : ?τ |- _ =>
     let lem := apply_canonical_form_lem τ in
     eapply lem in H; [ | solve [ eauto ] | solve [ eauto ] ]; try simp_hyp H
   end; subst.
-
-Ltac apply_canonical_form_weak_lem τ :=
-  lazymatch τ with
-  | <{ Π:{_}_, _ }> => canonical_form_weak_abs
-  | <{ 𝔹 }> => canonical_form_weak_bool
-  | <{ _ + _ }> => canonical_form_weak_sum
-  | <{ _ * _ }> => canonical_form_weak_prod
-  | <{ gvar _ }> => canonical_form_weak_fold
-  end.
-
-Ltac apply_canonical_form_weak :=
-  match goal with
-  | Hw : wval ?e, Ht : _; _ ⊢ ?e :{⊥} ?τ |- _ =>
-      eapply wval_val in Hw; [ | solve [ eauto ] ];
-      apply_canonical_form
-  | Hw : wval ?e, Ht : _; _ ⊢ ?e :{_} ?τ |- _ =>
-      let lem := apply_canonical_form_weak_lem τ in
-      eapply lem in Hw; [ | solve [ eauto ] | solve [ eauto ] ];
-      destruct Hw; try simp_hyp Hw; subst
-  end.
-
 
 Section fix_gctx.
 
@@ -272,15 +187,15 @@ Set Default Proof Using "Hwf".
 Ltac ctx_solver :=
   match goal with
   | |- exists _, _ ⊨ _ -->! _ =>
-    eexists; solve_ctx
+    eexists; solve_ectx
   end.
 
 (** The combined progress theorems for expressions and types. *)
 Theorem progress_ :
-  (forall Γ e l τ,
-      Γ ⊢ e :{l} τ ->
+  (forall Γ e τ,
+      Γ ⊢ e : τ ->
       Γ = ∅ ->
-      wval e \/ exists e', e -->! e') /\
+      val e \/ exists e', e -->! e') /\
   (forall Γ τ κ,
      Γ ⊢ τ :: κ ->
      Γ = ∅ ->
@@ -304,17 +219,17 @@ Proof.
       end;
     repeat
       match reverse goal with
-      | H : wval _ \/ exists _, _ |- _ =>
+      | H : val _ \/ exists _, _ |- _ =>
           destruct H as [| [] ]; [ | solve [ right; ctx_solver ] ]
       end;
-    try apply_canonical_form_weak;
-    try solve [ right; eauto using step, wval; ctx_solver
-              | left; eauto using wval, oval, otval ].
+    try apply_canonical_form;
+    try solve [ right; eauto using step, val; ctx_solver
+              | left; eauto using val, oval, otval ].
 
   (* Oblivious injection. It steps to boxed injection. *)
   right. otval_inv.
   repeat econstructor; eauto.
-  case_split; eauto using otval_well_kinded, val_oval, wval_val.
+  case_split; eauto using otval_well_kinded, val_oval.
 
   (* Oblivious case. *)
   right.
@@ -322,14 +237,10 @@ Proof.
   eauto using step.
 
   (* Oblivious pair. *)
-  left. eauto 10 using wval, oval, val_oval, wval_val.
-
-  (* Tape. *)
-  right.
-  hauto use: wval_woval ctrs: step inv: woval.
+  left. eauto 10 using val, oval, val_oval.
 
   (* Boxed injection. *)
-  left. qauto use: ovalty_elim ctrs: wval.
+  left. qauto use: ovalty_elim ctrs: val.
 
   (* Public product and sum. These case are impossible. *)
   1-2:  enough (<{ *@P }> ⊑ <{ *@O }>) by easy; scongruence use: join_ub_r.
@@ -338,18 +249,11 @@ Proof.
   select kind (fun κ => destruct κ); sintuition use: any_kind_otval.
 Qed.
 
-Theorem progress_weak l τ e :
-  ∅ ⊢ e :{l} τ ->
-  wval e \/ exists e', e -->! e'.
-Proof.
-  hauto use: progress_.
-Qed.
-
 Theorem progress τ e :
-  ∅ ⊢ e :{⊥} τ ->
+  ∅ ⊢ e : τ ->
   val e \/ exists e', e -->! e'.
 Proof.
-  hauto use: progress_, wval_val.
+  hauto use: progress_.
 Qed.
 
 Theorem kinding_progress τ :
